naming conventions

Cslib/Computability/LambdaCalculus/Untyped/LocallyNameless/Basic.lean
@@ -24,46 +24,46 @@ variable {Var : Type u} [HasFresh Var] [DecidableEq Var]
 
 namespace LambdaCalculus.LocallyNameless
 
-/-- Syntax of locally nameless lambda terms, with free variables over `Var`. -/
+/-- Syntax of locally nameless absbda terms, with free variables over `Var`. -/
 inductive Term (Var : Type u)
-/-- Bound variables that appear under a lambda abstraction, using a de-Bruijn index. -/
+/-- Bound variables that appear under a absbda abstraction, using a de-Bruijn index. -/
 | bvar : ℕ → Term Var
 /-- Free variables. -/
 | fvar : Var → Term Var
 /-- Lambda abstraction, introducing a new bound variable. -/
-| lam  : Term Var → Term Var
+| abs  : Term Var → Term Var
 /-- Function application. -/
 | app  : Term Var → Term Var → Term Var
 
 /-- Variable opening of the ith bound variable. -/
 @[simp]
-def Term.open_rec (i : ℕ) (sub : Term Var) : Term Var → Term Var
+def Term.openRec (i : ℕ) (sub : Term Var) : Term Var → Term Var
 | bvar i' => if i = i' then sub else bvar i'
 | fvar x  => fvar x
-| app l r => app (open_rec i sub l) (open_rec i sub r)
-| lam M   => lam $ open_rec (i+1) sub M
+| app l r => app (openRec i sub l) (openRec i sub r)
+| abs M   => abs $ openRec (i+1) sub M
 
-scoped notation:68 e "⟦" i " ↝ " sub "⟧"=> Term.open_rec i sub e 
+scoped notation:68 e "⟦" i " ↝ " sub "⟧"=> Term.openRec i sub e 
 
 /-- Variable opening of the closest binding. -/
 @[simp]
-def Term.open' {X} (e u):= @Term.open_rec X 0 u e
+def Term.open' {X} (e u):= @Term.openRec X 0 u e
 
 infixr:80 " ^ " => Term.open'
 
 /-- Variable closing, replacing a free `fvar x` with `bvar k` -/
 @[simp]
-def Term.close_rec (k : ℕ) (x : Var) : Term Var → Term Var
+def Term.closeRec (k : ℕ) (x : Var) : Term Var → Term Var
 | fvar x' => if x = x' then bvar k else fvar x'
 | bvar i  => bvar i
-| app l r => app (close_rec k x l) (close_rec k x r)
-| lam t   => lam $ close_rec (k+1) x t
+| app l r => app (closeRec k x l) (closeRec k x r)
+| abs t   => abs $ closeRec (k+1) x t
 
-scoped notation:68 e "⟦" k " ↜ " x "⟧"=> Term.close_rec k x e 
+scoped notation:68 e "⟦" k " ↜ " x "⟧"=> Term.closeRec k x e 
 
 /-- Variable closing of the closest binding. -/
 @[simp]
-def Term.close {Var} [DecidableEq Var] (e u):= @Term.close_rec Var _ 0 u e
+def Term.close {Var} [DecidableEq Var] (e u):= @Term.closeRec Var _ 0 u e
 
 infixr:80 " ^* " => Term.close
 
@@ -74,7 +74,7 @@ def Term.subst (m : Term Var) (x : Var) (sub : Term Var) : Term Var :=
   | bvar i  => bvar i
   | fvar x' => if x = x' then sub else fvar x'
   | app l r => app (l.subst x sub) (r.subst x sub)
-  | lam M   => lam $ M.subst x sub
+  | abs M   => abs $ M.subst x sub
 
 scoped notation:67 e "[" x ":=" sub "]" => Term.subst e x sub
 
@@ -83,11 +83,11 @@ scoped notation:67 e "[" x ":=" sub "]" => Term.subst e x sub
 def Term.fv : Term Var → Finset Var
 | bvar _ => {}
 | fvar x => {x}
-| lam e1 => e1.fv
+| abs e1 => e1.fv
 | app l r => l.fv ∪ r.fv
 
 /-- Locally closed terms. -/
 inductive Term.LC : Term Var → Prop
 | fvar (x)  : LC (fvar x)
-| lam (L : Finset Var) (e : Term Var) : (∀ x : Var, x ∉ L → LC (e ^ fvar x)) → LC (lam e)
+| abs (L : Finset Var) (e : Term Var) : (∀ x : Var, x ∉ L → LC (e ^ fvar x)) → LC (abs e)
 | app {l r} : l.LC → r.LC → LC (app l r)
